vale/code/arch/x64/interop/Fast_stdcalls.fsti
@@ -5,9 +5,14 @@ open FStar.HyperStack.ST
 module B = LowStar.Buffer
 module HS = FStar.HyperStack
 open Fast_defs
+open FStar.Mul
 
 unfold
 let u256 = b:B.buffer UInt64.t{B.length b == 4}
+unfold
+let u512 = b:B.buffer UInt64.t{B.length b == 8}
+unfold
+let u1024 = b:B.buffer UInt64.t{B.length b == 16}
 
 let as_nat (b:B.buffer UInt64.t{B.length b == 4}) (h:HS.mem) : GTot nat =
   let s = B.as_seq h b in
@@ -29,7 +34,7 @@ val add1
   (ensures fun h0 c h1 ->
     B.live h1 out /\ B.live h1 f1 /\
     B.modifies (B.loc_buffer out) h0 h1 /\
-    as_nat out h1 + pow2_256 `op_Multiply` UInt64.v c == as_nat f1 h0 + UInt64.v f2)  
+    as_nat out h1 + pow2_256 * UInt64.v c == as_nat f1 h0 + UInt64.v f2)  
 
 val fadd
   (out:u256)
@@ -60,3 +65,24 @@ val fsub
     (ensures  fun h0 _ h1 ->
       B.modifies (B.loc_buffer out) h0 h1 /\
       (as_nat out h1) % prime == (as_nat f1 h0 - as_nat f2 h0) % prime)
+
+val fmul 
+  (tmp:u512)
+  (f1:u256)
+  (out:u256) 
+  (f2:u256)
+  : Stack unit
+    (requires fun h -> 
+      adx_enabled /\ bmi2_enabled /\
+      B.live h out /\ B.live h f1 /\ B.live h f2 /\ B.live h tmp /\
+      (B.disjoint out f1 \/ out == f1) /\
+      (B.disjoint out f2 \/ out == f2) /\
+      (B.disjoint out tmp \/ out == tmp) /\
+      (B.disjoint f1 f2 \/ f1 == f2) /\
+      B.disjoint f1 tmp /\
+      B.disjoint f2 tmp
+    )
+    (ensures  fun h0 _ h1 ->
+      B.modifies (B.loc_union (B.loc_buffer out) (B.loc_buffer tmp)) h0 h1 /\
+      (as_nat out h1) % prime == (as_nat f1 h0 * as_nat f2 h0) % prime)
+ 
